Impl/EvictModel.i.dfy
@@ -2,7 +2,7 @@ include "DeallocModel.i.dfy"
 include "SyncModel.i.dfy"
 
 module ImplModelEvict {
-  import opened ImplModel
+  import opened StateModel
   import opened ImplModelIO
   import opened ImplModelCache
   import opened ImplModelDealloc
