Impl/Mkfs.i.dfy
@@ -1,6 +1,6 @@
 include "Marshalling.i.dfy"
 include "Impl.i.dfy"
-include "ImplState.i.dfy"
+include "StateImpl.i.dfy"
 include "ImplMarshalling.i.dfy"
 
 // TODO make separate spec abstract module
@@ -11,7 +11,7 @@ module {:extern} MkfsImpl {
   import opened NativeTypes
   import opened Impl
   import opened BucketWeights
-  import IM = ImplModel
+  import SM = StateModel
   import opened MutableBucket
   import opened ImplNode
   import KVList
@@ -41,7 +41,7 @@ module {:extern} MkfsImpl {
     WeightBucketListOneEmpty();
     assert node.I().buckets == [empty.I()];    // OBSERVE (trigger)
     ghost var sector:IS.Sector := IS.SectorBlock(node);
-    ghost var is:IM.Sector := IS.ISector(sector);
+    ghost var is:SM.Sector := IS.ISector(sector);
     var b1 := ImplMarshalling.MarshallCheckedSector(IS.SectorBlock(node));
 
     var sectorIndirectionTable := new IndirectionTableImpl.IndirectionTable.Empty();
@@ -53,13 +53,13 @@ module {:extern} MkfsImpl {
     // Need to improve the contract between sectorIndirectionTable and here.
     assume sectorIndirectionTable.Inv();
 
-    assume IM.IIndirectionTable(IS.IIndirectionTable(sectorIndirectionTable)) == BC.IndirectionTable(
+    assume SM.IIndirectionTable(IS.IIndirectionTable(sectorIndirectionTable)) == BC.IndirectionTable(
       map[0 := LBAType.Location(LBAType.BlockSize(), b1.Length as uint64)],
       map[0 := []]
     );
 
     //assert IS.WFSector(IS.SectorIndirectionTable(sectorIndirectionTable));
-    assume IM.WFSector(IS.ISector(IS.SectorIndirectionTable(sectorIndirectionTable)));
+    assume SM.WFSector(IS.ISector(IS.SectorIndirectionTable(sectorIndirectionTable)));
     var b0 := ImplMarshalling.MarshallCheckedSector(IS.SectorIndirectionTable(sectorIndirectionTable));
 
     // TODO(jonh): MarshallCheckedSector owes us a promise that it can marshall
